Checkpoint progress on recovery adequacy proof.

src/program_logic/recovery_adequacy.v
@@ -144,31 +144,35 @@ End crash_adequacy.
 
 (*** Recovery ***)
 
-Class pbundleG (T: ofeT) := {
+Class pbundleG (T: ofeT) (Σ: gFunctors) := {
   pbundleT : T
 }.
 
-Class perennialG (Λ : language) (CS: crash_semantics Λ) (T: ofeT) (Σ : gFunctors) := IrisG {
-  perennial_irisG :> pbundleG T → irisG Λ Σ;
+Class perennialG (Λ : language) (CS: crash_semantics Λ) (T: ofeT) (Σ : gFunctors) := PerennialG {
+  perennial_irisG :> ∀ H, pbundleG T Σ → irisG Λ Σ;
+  perennial_invG: ∀ H t, @iris_invG _ _ (perennial_irisG H t) = H
 }.
 
+Print wp_pre.
+
 Definition wpr_pre `{perennialG Λ CS T Σ} (s : stuckness)
-    (wpr : pbundleG T -d> coPset -d> expr Λ -d> expr Λ -d> (val Λ -d> iPropO Σ) -d> (pbundleG T -d> val Λ -d> iPropO Σ) -d> iPropO Σ) :
-  pbundleG T -d> coPset -d> expr Λ -d> expr Λ -d> (val Λ -d> iPropO Σ) -d> (pbundleG T -d> val Λ -d> iPropO Σ) -d> iPropO Σ :=
-  λ t E e rec Φ Φr,
+    (wpr : invG Σ -d> pbundleG T Σ -d> coPset -d> expr Λ -d> expr Λ -d> (val Λ -d> iPropO Σ) -d>
+                     (invG Σ -d> pbundleG T Σ -d> val Λ -d> iPropO Σ) -d> iPropO Σ) :
+  invG Σ -d> pbundleG T Σ -d> coPset -d> expr Λ -d> expr Λ -d> (val Λ -d> iPropO Σ) -d> (invG Σ -d> pbundleG T Σ -d> val Λ -d> iPropO Σ) -d> iPropO Σ :=
+  λ H t E e rec Φ Φr,
   (WPC e @ s ; E ; ∅
      {{ Φ }}
      {{ ∀ σ σ' (HC: crash_prim_step CS σ σ') κs n,
-        state_interp σ κs n ={∅}=∗  ▷ ∃ t, state_interp σ' κs 0 ∗ wpr t E rec rec (λ v, Φr t v) Φr}})%I.
+        state_interp σ κs n ={∅}=∗  ▷ ∀ H, ∃ t, state_interp σ' κs 0 ∗ wpr H t E rec rec (λ v, Φr H t v) Φr}})%I.
 
 Local Instance wpr_pre_contractive `{!perennialG Λ CS T Σ} s : Contractive (wpr_pre s).
 Proof.
-  rewrite /wpr_pre=> n wp wp' Hwp t E1 e1 rec Φ Φc.
+  rewrite /wpr_pre=> n wp wp' Hwp ? t E1 e1 rec Φ Φc.
   repeat (f_contractive || f_equiv); apply Hwp.
 Qed.
 
 Definition wpr_def `{!perennialG Λ CS T Σ} (s : stuckness) :
-  pbundleG T → coPset → expr Λ → expr Λ → (val Λ → iProp Σ) → (pbundleG T → val Λ → iProp Σ) → iProp Σ := fixpoint (wpr_pre s).
+  invG Σ → pbundleG T Σ → coPset → expr Λ → expr Λ → (val Λ → iProp Σ) → (invG Σ → pbundleG T Σ → val Λ → iProp Σ) → iProp Σ := fixpoint (wpr_pre s).
 Definition wpr_aux `{!perennialG Λ CS T Σ} : seal (@wpr_def Λ CS T Σ _). by eexists. Qed.
 Definition wpr `{!perennialG Λ CS T Σ} := wpr_aux.(unseal).
 Definition wpr_eq `{!perennialG Λ CS T Σ} : wpr = @wpr_def Λ CS T Σ _ := wpr_aux.(seal_eq).
@@ -178,51 +182,51 @@ Context `{!perennialG Λ CS T Σ}.
 Implicit Types s : stuckness.
 Implicit Types P : iProp Σ.
 Implicit Types Φ : val Λ → iProp Σ.
-Implicit Types Φc : pbundleG T → val Λ → iProp Σ.
+Implicit Types Φc : invG Σ → pbundleG T Σ → val Λ → iProp Σ.
 Implicit Types v : val Λ.
 Implicit Types e : expr Λ.
 
-Lemma wpr_unfold s t E e rec Φ Φc :
-  wpr s t E e rec Φ Φc ⊣⊢ wpr_pre s (wpr s) t E e rec Φ Φc.
+Lemma wpr_unfold s Hi t E e rec Φ Φc :
+  wpr s Hi t E e rec Φ Φc ⊣⊢ wpr_pre s (wpr s) Hi t E e rec Φ Φc.
 Proof. rewrite wpr_eq. apply (fixpoint_unfold (wpr_pre s)). Qed.
 
 (* There's a stronger version of this *)
-Lemma wpr_strong_mono s t E e rec Φ Ψ Φr Ψr :
-  wpr s t E e rec Φ Φr -∗
-  (∀ v, Φ v ==∗ Ψ v) ∧ (∀ t v, Φr t v ==∗ Ψr t v) -∗
-  wpr s t E e rec Ψ Ψr.
+Lemma wpr_strong_mono s Hi t E e rec Φ Ψ Φr Ψr :
+  wpr s Hi t E e rec Φ Φr -∗
+  (∀ v, Φ v ==∗ Ψ v) ∧ (∀ Hi t v, Φr Hi t v ==∗ Ψr Hi t v) -∗
+  wpr s Hi t E e rec Ψ Ψr.
 Proof.
-  iIntros "H HΦ". iLöb as "IH" forall (e t E Φ Ψ Φr Ψr).
+  iIntros "H HΦ". iLöb as "IH" forall (e t Hi E Φ Ψ Φr Ψr).
   rewrite ?wpr_unfold /wpr_pre.
   iApply (wpc_strong_mono with "H") ; auto.
   iSplit.
   { iDestruct "HΦ" as "(H&_)". iIntros. iMod ("H" with "[$]"); eauto. }
   iIntros "H".
   iModIntro. iIntros (?????) "Hinterp". iMod ("H" with "[//] Hinterp") as "H".
-  iModIntro. iNext. iDestruct "H" as (?) "(?&H)".
+  iModIntro. iNext. iIntros (Hi'). iDestruct ("H" $! Hi') as (?) "(?&H)".
   iExists _. iFrame. iApply ("IH" with "[$]").
   iSplit; iIntros; iDestruct ("HΦ") as "(_&H)"; by iMod ("H" with "[$]").
 Qed.
 
 (* To prove a recovery wp for e with rec, it suffices to prove a crash wp for e,
    where the crash condition implies the precondition for a crash wp for rec *)
-Lemma idempotence_wpr s E e rec Φx Φrx Φcx t:
+Lemma idempotence_wpr s E e rec Φx Φrx Φcx Hi t:
   ((WPC e @ s ; E ; ∅ {{ Φx t }} {{ Φcx t }}) -∗
-   (□ ∀ (t: pbundleG T) σ σ' (HC: crash_prim_step CS σ σ') κs n,
+   (□ ∀ (H: invG Σ) (t: pbundleG T Σ) σ σ' (HC: crash_prim_step CS σ σ') κs n,
         Φcx t -∗ state_interp σ κs n ={∅}=∗
-        ▷ ∃ t', state_interp σ' κs 0 ∗ WPC rec @ s ; E ; ∅ {{ Φrx t' }} {{ Φcx t' }}) -∗
-    wpr s t E e rec (Φx t) Φrx)%I.
+        ▷ ∀ H', ∃ t', state_interp σ' κs 0 ∗ WPC rec @ s ; E ; ∅ {{ Φrx H' t' }} {{ Φcx t' }}) -∗
+    wpr s Hi t E e rec (Φx t) Φrx)%I.
 Proof.
-  iLöb as "IH" forall (E e t Φx).
+  iLöb as "IH" forall (E e Hi t Φx).
   iIntros "He #Hidemp".
   rewrite wpr_unfold. rewrite /wpr_pre.
   iApply (wpc_strong_mono with "He"); [ auto | auto | auto | ].
   iSplit; first auto. iIntros "Hcx". iModIntro.
   iIntros. iMod ("Hidemp" with "[ ] [$] [$]") as "H".
   { eauto. }
-  iModIntro. iNext. iDestruct "H" as (t') "(?&Hc)".
+  iModIntro. iNext. iIntros (Hi'). iDestruct ("H" $! Hi') as (t') "(?&Hc)".
   iExists _. iFrame.
-  iApply ("IH" $! E rec t' (λ t v, Φrx t v)%I with "[Hc]").
+  iApply ("IH" $! E rec Hi' t' (λ t v, Φrx Hi' t v)%I with "[Hc]").
   { iApply (wpc_strong_mono with "Hc"); auto. }
   eauto.
 Qed.
@@ -234,16 +238,16 @@ Context `{!perennialG Λ CS T Σ}.
 Implicit Types s : stuckness.
 Implicit Types P : iProp Σ.
 Implicit Types Φ : val Λ → iProp Σ.
-Implicit Types Φc : pbundleG T → iProp Σ.
+Implicit Types Φc : invG Σ → pbundleG T Σ → val Λ → iProp Σ.
 Implicit Types v : val Λ.
 Implicit Types e : expr Λ.
 
 Notation wptp s t := ([∗ list] ef ∈ t, WPC ef @ s; ⊤; ∅ {{ fork_post }} {{ True }})%I.
 
-Lemma wptp_recv_strong_adequacy Φ Φr κs' s t n ns r1 e1 t1 κs t2 σ1 σ2 :
+Lemma wptp_recv_strong_adequacy Φ Φr κs' s Hi t n ns r1 e1 t1 κs t2 σ1 σ2 :
   nrsteps (CS := CS) r1 (n :: ns) (e1 :: t1, σ1) κs (t2, σ2) Normal →
   state_interp σ1 (κs ++ κs') (length t1) -∗
-  wpr s t ⊤ e1 r1 Φ Φr -∗
+  wpr s Hi t ⊤ e1 r1 Φ Φr -∗
   wptp s t1 ={⊤,∅}▷=∗^(S n) (∃ e2 t2',
     ⌜ t2 = e2 :: t2' ⌝ ∗
     ⌜ ∀ e2, s = NotStuck → e2 ∈ t2 → (is_Some (to_val e2) ∨ reducible e2 σ2) ⌝ ∗
@@ -253,17 +257,165 @@ Lemma wptp_recv_strong_adequacy Φ Φr κs' s t n ns r1 e1 t1 κs t2 σ1 σ2 :
 Proof.
   iIntros (Hstep) "Hσ He Ht".
   inversion Hstep. subst.
-  iApply (wptp_strong_adequacy with "[$] [He]"); eauto.
-  rewrite wpr_unfold /wpr_pre. iApply "He".
+  iPoseProof (wptp_strong_adequacy with "Hσ [He] Ht") as "H".
+  { eauto. }
+  {rewrite wpr_unfold /wpr_pre. iApply "He". }
+  rewrite perennial_invG.
+  iApply "H".
 Qed.
 
-Fixpoint step_fupdN_fresh (ns: list nat) t0 (P: pbundleG T → iProp Σ) :=
+Fixpoint fupd_fresh (ns: list nat) Hi0 (P: invG Σ → iProp Σ) :=
   match ns with
-  | [] => P t0
+  | [] => P Hi0
+  | (n :: ns) =>
+    (|={⊤}=> ∀ Hi', fupd_fresh ns Hi' P)%I
+  end.
+
+Fixpoint step_fupdN_fresh (ns: list nat) Hi0 t0 (P: invG Σ → pbundleG T Σ → iProp Σ) :=
+  match ns with
+  | [] => P Hi0 t0
   | (n :: ns) =>
     (|={⊤, ∅}▷=>^(S n) |={⊤, ∅}=> ▷
-     (∃ t' : pbundleG T, step_fupdN_fresh ns t' P))%I
+     ∀ Hi', (∃ t' : pbundleG T Σ, step_fupdN_fresh ns Hi' t' P))%I
   end.
+
+
+Lemma step_fupdN_fresh_snoc (ns: list nat) n Hi0 t0 Q:
+  step_fupdN_fresh (ns ++ [n]) Hi0 t0 Q ≡
+  step_fupdN_fresh (ns) Hi0 t0 (λ Hi _, |={⊤, ∅}▷=>^(S n) |={⊤, ∅}=> ▷ ∀ Hi', ∃ t', Q Hi' t')%I.
+Proof.
+  apply (anti_symm (⊢)%I).
+  - revert Hi0 t0 Q.
+    induction ns => ??? //=. do 3 f_equiv.
+    apply step_fupdN_mono.
+    do 2 f_equiv. do 2 (f_equiv => ?).
+    rewrite IHns. eauto.
+  - revert Hi0 t0 Q.
+    induction ns => ??? //=. do 3 f_equiv.
+    apply step_fupdN_mono.
+    do 2 f_equiv. do 2 (f_equiv => ?).
+    rewrite IHns. eauto.
+Qed.
+
+Lemma step_fupdN_fresh_pattern_wand {H: invG Σ} n (Q Q': iProp Σ):
+  (|={⊤, ∅}▷=>^(S n) |={⊤, ∅}=> ▷ Q) -∗ (Q -∗ Q') -∗
+  (|={⊤, ∅}▷=>^(S n) |={⊤, ∅}=> ▷ Q').
+Proof.
+  iIntros "H Hwand". simpl.
+  iApply (step_fupdN_wand with "H").
+  iNext. iIntros "H".
+  iMod "H". iModIntro. iNext.
+  by iApply "Hwand".
+Qed.
+
+Lemma step_fupdN_fresh_pattern_plain {H: invG Σ} n (Q: iProp Σ) `{!Plain Q}:
+  (|={⊤, ∅}▷=>^(S n) |={⊤, ∅}=> ▷ Q)-∗
+  (|={⊤}=> ▷^(S (S n)) Q).
+Proof.
+  iIntros "H".
+  iDestruct (step_fupdN_wand with "H []") as "H".
+  { iApply fupd_plain_mask_empty. }
+  rewrite -step_fupdN_S_fupd.
+  iDestruct (step_fupdN_plain with "H") as "H".
+  iMod "H". iModIntro. iNext. rewrite -later_laterN laterN_later. iNext. by iMod "H".
+Qed.
+
+Lemma step_fupdN_fresh_wand (ns: list nat) Hi0 t0 Q Q':
+  step_fupdN_fresh (ns) Hi0 t0 Q -∗ (∀ Hinv t, Q Hinv t -∗ Q' Hinv t)
+  -∗ step_fupdN_fresh ns Hi0 t0 Q'.
+Proof.
+  revert Hi0 t0.
+  induction ns => ??.
+  - iIntros "H Hwand". iApply "Hwand". eauto.
+  - iIntros "H Hwand". simpl.
+    iApply (step_fupdN_fresh_pattern_wand with "H [Hwand]").
+    iIntros "H".
+    iIntros (Hi'). iSpecialize ("H" $! Hi'). iDestruct "H" as (?) "H".
+    iExists _. iApply (IHns with "H"). eauto.
+Qed.
+
+Lemma step_fupdN_fresh_snoc_plain ns n Hinv t0 P `{!Plain P}:
+  step_fupdN_fresh (ns ++ [n]) Hinv t0 (λ (x : invG Σ) (t : pbundleG T Σ), P) -∗
+  step_fupdN_fresh ns Hinv t0 (λ (x : invG Σ) (t : pbundleG T Σ), |={⊤}=> ▷^(S (S n)) P).
+Proof.
+  iIntros "H".
+  rewrite ?step_fupdN_fresh_snoc.
+  iApply (step_fupdN_fresh_wand with "H").
+  { iIntros (Hinv' ?) "H".
+   iDestruct (step_fupdN_wand _ _ _ _ (|={⊤}=> ▷ P)%I with "H []") as "H'".
+   { iIntros "H". iApply fupd_plain_mask_empty.  iMod "H". iModIntro.
+     iNext. iDestruct ("H" $! Hinv') as (_) "$". }
+   rewrite -step_fupdN_S_fupd.
+   iMod (step_fupdN_plain with "H'") as "Hφ". iModIntro. simpl. iNext.
+   rewrite -later_laterN laterN_later.
+   iNext. by iMod "Hφ".
+  }
+Qed.
+
+Lemma fupd_fresh_plain_1 `{!invPreG Σ} P `{!Plain P} ns:
+  (∀ Hinv', fupd_fresh ns Hinv' (λ _, P)) ==∗ ◇ P.
+Proof.
+  iIntros "H".
+  iInduction ns as [| n ns] "IH".
+  - simpl. iMod wsat_alloc as (Hinv) "(Hw&HE)". iApply ("H" $! Hinv).
+  - iMod wsat_alloc as (Hinv) "(Hw&HE)".
+    iSpecialize ("H" $! Hinv).
+    simpl.
+    rewrite uPred_fupd_eq /uPred_fupd_def.
+    iMod ("H" with "[$]") as "[Hw [HE H]]".
+    iMod "H". by iApply "IH".
+Qed.
+
+Fixpoint fresh_later_count (ns: list nat) :=
+  match ns with
+  | [] => 2
+  | n :: ns' => (S (S n)) + fresh_later_count ns'
+  end.
+
+Lemma step_fupdN_fresh_plain `{!invPreG Σ} P `{!Plain P} ns:
+  (∀ Hinv', ∃ t, step_fupdN_fresh ns Hinv' t (λ _ _, P)) -∗ ▷^(fresh_later_count ns) P.
+Proof.
+  iIntros "H".
+  iInduction ns as [| n' ns] "IH".
+  - simpl. iApply bupd_plain; first by (iPureIntro; apply _).
+    iMod wsat_alloc as (Hinv) "(Hw&HE)". by iDestruct ("H" $! Hinv) as (_) "$".
+  - iMod wsat_alloc as (Hinv) "(Hw&HE)".
+    iSpecialize ("H" $! Hinv).
+    iDestruct "H" as (t) "H".
+    rewrite /step_fupdN_fresh -/step_fupdN_fresh.
+    iDestruct (step_fupdN_fresh_pattern_wand with "H IH") as "H".
+    iDestruct (step_fupdN_fresh_pattern_plain with "H") as "H".
+    rewrite {1}uPred_fupd_eq {1}/uPred_fupd_def.
+    iMod ("H" with "[$]") as "[Hw [HE >H]]".
+    by rewrite laterN_plus.
+Qed.
+
+Lemma fupd_fresh_plain_soundness `{!invPreG Σ} (P: iProp Σ) `{!Plain P} ns:
+  (∀ `{Hinv: !invG Σ}, bi_emp_valid (fupd_fresh ns Hinv (λ _, P))) → bi_emp_valid P.
+Proof.
+  iIntros (Hfupd).
+  apply later_soundness.
+  iAssert (∀ Hinv, fupd_fresh ns Hinv (λ _: invG Σ, P))%I as "H".
+  { iIntros. iApply Hfupd. }
+  clear Hfupd.
+  iInduction ns as [| n ns] "IH".
+  - simpl. iMod wsat_alloc as (Hinv) "_". iApply ("H" $! Hinv).
+  - iMod wsat_alloc as (Hinv) "[Hw HE]".
+    iSpecialize ("H" $! Hinv).
+    simpl.
+    rewrite uPred_fupd_eq /uPred_fupd_def.
+    iMod ("H" with "[$]") as "[Hw [HE >H']]".
+    iApply ("IH" with "H'").
+Qed.
+
+Lemma step_fupdN_fresh_soundness' `{!invPreG Σ} (φ : Prop) ns:
+  (∀ Hinv : invG Σ, (∃ t0, step_fupdN_fresh ns Hinv t0 (λ _ _, ⌜φ⌝))%I) →
+  φ.
+Proof.
+  intros Hiter.
+  apply (soundness (M:=iResUR Σ) _  (fresh_later_count ns)); simpl.
+  iApply step_fupdN_fresh_plain. iIntros (Hinv). iApply Hiter.
+Qed.
 
 (*
 Notation "|={ E }=>_( t ) Q" := (fupd (FUpd := t) E E Q)
@@ -272,19 +424,69 @@ Notation "P ={ E }=∗_ t Q" := (P -∗ |={E}=>_(t) Q)%I
  (at level 99) : bi_scope.
 *)
 
-Lemma wptp_recv_strong_crash_adequacy Φ Φr κs' s t ns r1 e1 t1 κs t2 σ1 σ2 :
-  nrsteps (CS := CS) r1 ns (e1 :: t1, σ1) κs (t2, σ2) Crashed →
+(*
+Lemma wptp_recv_strong_crash_adequacy Φ Φr κs' s Hi t ns n r1 e1 t1 κs t2 σ1 σ2 :
+  nrsteps (CS := CS) r1 (ns ++ [n]) (e1 :: t1, σ1) κs (t2, σ2) Crashed →
   state_interp σ1 (κs ++ κs') (length t1) -∗
-  wpr s t ⊤ e1 r1 Φ Φr -∗
-  wptp s t1 -∗ step_fupdN_fresh ns t (λ t', ∃ e2 t2',
+  wpr s Hi t ⊤ e1 r1 Φ Φr -∗
+  wptp s t1 -∗ step_fupdN_fresh ns Hi t (λ Hi' t',
+    (|={⊤, ∅}▷=>^(S n) |={⊤, ∅}=> ▷ ∃ e2 t2',
     ⌜ t2 = e2 :: t2' ⌝ ∗
     ⌜ ∀ e2, s = NotStuck → e2 ∈ t2 → (is_Some (to_val e2) ∨ reducible e2 σ2) ⌝ ∗
     state_interp σ2 κs' (length t2') ∗
-    from_option (Φr t') True (to_val e2) ∗
+    from_option (Φr Hi' t') True (to_val e2) ∗
+    ([∗ list] v ∈ omap to_val t2', fork_post v))).
+Proof.
+  revert Hi t e1 t1 κs κs' t2 σ1 σ2 Φ.
+  induction ns as [|n' ns' IH] => Hi t e1 t1 κs κs' t2 σ1 σ2 Φ.
+  (*
+  { inversion_clear 1. }
+   *)
+  iIntros (Hsteps) "Hσ He Ht".
+  inversion_clear Hsteps as [|?? [t1' σ1'] ????? s0].
+  rewrite {1}/step_fupdN_fresh -/step_fupdN_fresh.
+  destruct ρ2 as (?&σ2_pre_crash).
+  iApply (step_fupdN_wand with "[-]").
+  { rewrite -assoc wpr_unfold /wpr_pre.
+    iPoseProof (@wptp_strong_crash_adequacy with "[$] [$]") as "H"; eauto.
+    rewrite perennial_invG. by iApply "H".
+  }
+  iIntros "H". iMod "H" as (e2 t2' ?) "(H&Hσ)".
+  iMod ("H" with "[//] Hσ") as "H". iModIntro. iNext.
+  destruct s0.
+  - iIntros (Hi'). iSpecialize ("H" $! Hi').
+    iDestruct "H" as (t') "(Hσ&Hr)".
+    iPoseProof (IH with "[Hσ] Hr []") as "H"; eauto.
+  - iIntros (Hi').
+    iDestruct ("H" $! Hi') as (t') "(Hσ&Hr)".
+    iExists t'. subst. inversion H1; subst.
+    rewrite /step_fupdN_fresh.
+    iPoseProof (wptp_strong_adequacy with "[Hσ] [Hr] []") as "H"; eauto.
+    { rewrite wpr_unfold /wpr_pre. iApply "Hr". }
+    rewrite perennial_invG.
+    iApply (step_fupdN_wand with "H").
+    iIntros "H". iDestruct "H" as (????) "(Hσ&?&?)".
+    iApply (fupd_mask_weaken _ ∅); first by set_solver+.
+    iNext. iIntros (Hi''). iExists t', _, _. iFrame.
+    iSplitL ""; eauto. (* *)
+Abort.
+*)
+
+
+(* XXX: Use of step_fupdN_fresh modality here does "an extra" crash *)
+Lemma wptp_recv_strong_crash_adequacy Φ Φr κs' s Hi t ns r1 e1 t1 κs t2 σ1 σ2 :
+  nrsteps (CS := CS) r1 ns (e1 :: t1, σ1) κs (t2, σ2) Crashed →
+  state_interp σ1 (κs ++ κs') (length t1) -∗
+  wpr s Hi t ⊤ e1 r1 Φ Φr -∗
+  wptp s t1 -∗ step_fupdN_fresh ns Hi t (λ Hi' t', ∃ e2 t2',
+    ⌜ t2 = e2 :: t2' ⌝ ∗
+    ⌜ ∀ e2, s = NotStuck → e2 ∈ t2 → (is_Some (to_val e2) ∨ reducible e2 σ2) ⌝ ∗
+    state_interp σ2 κs' (length t2') ∗
+    from_option (Φr Hi' t') True (to_val e2) ∗
     ([∗ list] v ∈ omap to_val t2', fork_post v)).
 Proof.
-  revert t e1 t1 κs κs' t2 σ1 σ2 Φ.
-  induction ns as [|n ns' IH] => t e1 t1 κs κs' t2 σ1 σ2 Φ.
+  revert Hi t e1 t1 κs κs' t2 σ1 σ2 Φ.
+  induction ns as [|n ns' IH] => Hi t e1 t1 κs κs' t2 σ1 σ2 Φ.
   { inversion_clear 1. }
   iIntros (Hsteps) "Hσ He Ht".
   inversion_clear Hsteps as [|?? [t1' σ1'] ????? s0].
@@ -292,23 +494,31 @@ Proof.
   destruct ρ2 as (?&σ2_pre_crash).
   iApply (step_fupdN_wand with "[-]").
   { rewrite -assoc wpr_unfold /wpr_pre.
-    iApply (wptp_strong_crash_adequacy with "[$] [$]"); eauto.
+    iPoseProof (@wptp_strong_crash_adequacy with "[$] [$]") as "H"; eauto.
+    rewrite perennial_invG. by iApply "H".
   }
   iIntros "H". iMod "H" as (e2 t2' ?) "(H&Hσ)".
   iMod ("H" with "[//] Hσ") as "H". iModIntro. iNext.
-  iDestruct "H" as (t') "(Hσ&Hr)".
   destruct s0.
-  - iPoseProof (IH with "[Hσ] Hr []") as "H"; eauto.
-  - iExists t'. subst. inversion H1; subst.
+  - iIntros (Hi'). iSpecialize ("H" $! Hi').
+    iDestruct "H" as (t') "(Hσ&Hr)".
+    iPoseProof (IH with "[Hσ] Hr []") as "H"; eauto.
+  - iIntros (Hi').
+    iDestruct ("H" $! Hi') as (t') "(Hσ&Hr)".
+    iExists t'. subst. inversion H1; subst.
     rewrite /step_fupdN_fresh.
     iPoseProof (wptp_strong_adequacy with "[Hσ] [Hr] []") as "H"; eauto.
     { rewrite wpr_unfold /wpr_pre. iApply "Hr". }
+    rewrite perennial_invG.
     iApply (step_fupdN_wand with "H").
     iIntros "H". iDestruct "H" as (????) "(Hσ&?&?)".
     iApply (fupd_mask_weaken _ ∅); first by set_solver+.
-    iNext. iExists t', _, _. iFrame.
-    iSplitL ""; eauto.
+    iNext. iIntros (Hi''). iExists t', _, _. iFrame.
+    iSplitL ""; eauto. (* *)
+Abort.
+(*
 Qed.
+*)
 End recovery_adequacy.
 
 Record recv_adequate {Λ CS} (s : stuckness) (e1 r1: expr Λ) (σ1 : state Λ)
@@ -324,3 +534,34 @@ Record recv_adequate {Λ CS} (s : stuckness) (e1 r1: expr Λ) (σ1 : state Λ)
    erased_rsteps (CS := CS) r1 ([e1], σ1) (t2, σ2) stat →
    e2 ∈ t2 → (is_Some (to_val e2) ∨ reducible e2 σ2)
 }.
+
+(*
+Corollary wp_recv_adequacy Σ Λ CS (T: ofeT) `{!invPreG Σ} s e r σ φ φr :
+  (∀ `{Hinv : !invG Σ} κs,
+     (|={⊤}=> ∃ (t: pbundleG T)
+         (invT: pbundleG T → invG Σ)
+         (stateI : pbundleG T → state Λ → list (observation Λ) → iProp Σ)
+         (fork_post : pbundleG T → val Λ → iProp Σ),
+        let _ : perennialG Λ CS _ Σ :=
+            PerennialG _ _ T Σ
+              (λ t,
+               IrisG Λ Σ (invT t) (λ σ κs _, stateI t σ κs)
+                    (fork_post t))
+               in
+       stateI t σ κs ∗ wpr s t ⊤ e r (λ v, ⌜φ v⌝) (λ _ v, ⌜φr v⌝))%I) →
+  recv_adequate (CS := CS) s e r σ (λ v _, φ v) (λ v _, φr v) .
+Proof.
+  intros Hwp. split.
+  - intros t2 σ2 v2 [n [κs ?]]%erased_rsteps_nrsteps.
+    eapply (step_fupdN_soundness' _ (S (S n)))=> Hinv. rewrite Nat_iter_S.
+  eapply (wp_recv_strong_adequacy Σ _); [|done]=> ?.
+  econstructor. apply adequate_alt; intros t2 σ2 [n [κs ?]]%erased_steps_nsteps.
+  eapply (wp_strong_adequacy Σ _); [|done]=> ?.
+  iMod Hwp as (stateI fork_post) "[Hσ Hwp]".
+  iExists s, (λ σ κs _, stateI σ κs), (λ v, ⌜φ v⌝%I), fork_post.
+  iIntros "{$Hσ $Hwp} !>" (e2 t2' -> ?) "_ H _".
+  iApply fupd_mask_weaken; [done|]. iSplit; [|done].
+  iIntros (v2 t2'' [= -> <-]). by rewrite to_of_val.
+Qed.
+
+*)
